theories/lang/cpp/semantics/subtyping.v
@@ -18,30 +18,40 @@ Require Import bedrock.lang.cpp.semantics.genv.
 Section extends.
   Context (σ : genv).
 
-  (** [class_derives mdc cls] is a/the proof that [mdc] is a derived class
-      of [cls] (equivalently, [cls] is a base class of [mdc])
-
-      note that this definition is in [Set] allowing us to compute over it.
+  (** [class_derives σ derived path]
+      - [derived] is the most derived class name
+      - [path] is the path from the most-derived class (head of the list)
+        to the base class (end of the list)
+      An example,
+      ```c++
+      class A {};
+      class B : public A {};
+      class C : public B {};
+      ```
+      the following hold:
+      - [class_derives "::A" []], [class_derives "::B" []], [class_derives "::C" []]
+      - [class_derives "::B" ["::A"]], [class_derives "::C" ["::B"]]
+      - [class_derives "::C" ["::B","::A"]]
    *)
-  Inductive class_derives (derived : globname) : globname -> Set :=
+  Inductive class_derives (derived : globname) : list globname -> Prop :=
   | Derives_here {st}
       {_ : σ.(genv_tu) !! derived = Some (Gstruct st)}
-    : class_derives derived derived
+    : class_derives derived []
 
-  | Derives_base base {st li result}
+  | Derives_base {base st li rest}
       {_ : σ.(genv_tu) !! derived = Some (Gstruct st)}
-      {_ : In (base, li) st.(s_bases)}
-      (_ : class_derives base result)
-    : class_derives derived result
+      {_ : (base, li) ∈ st.(s_bases)}
+      (_ : class_derives base rest)
+    : class_derives derived (base :: rest)
 
-  (* this could be extended for virtuals *)
+  (* this does not currently support `virtual` inheritence. *)
   .
 
 End extends.
 
 Arguments Derives_here {_ _} _ _.
 Arguments Derives_base {_ _} _.
-Arguments class_derives σ derived base : rename.
+Arguments class_derives {σ} derived path : rename.
 
 (** The following instances enable TC resolution to prove
 [class_derives σ derived base] when the translation unit [tu] and
@@ -52,24 +62,63 @@ that's presumably faster. *)
 Existing Class class_derives.
 #[global] Hint Mode class_derives - + + : typeclass_instances.
 
+Section tu.
+  Variable tu : translation_unit.
+
+  Fixpoint tu_class_derives (cls : globname) (path : list globname) : bool :=
+    match tu !! cls with
+    | Some (Gstruct st) =>
+        match path with
+        | nil => true
+        | base :: rest =>
+            if bool_decide (base ∈ (fst <$> st.(s_bases))) then
+              tu_class_derives base rest
+            else false
+        end
+    | _ => false
+    end.
+
+(*
+  Context {σ : genv} {M : tu ⊧ σ}.
+  Theorem tu_class_derives_sound : forall path,
+      tu_class_derives path -> class_derives σ path.
+  Proof using M.
+    induction path =>///=.
+    case_match.
+    { repeat case_match => //.
+      apply glob_def_genv_compat_struct in Heqo.
+      intro.
+      econstructor. eassumption. }
+    { repeat (case_bool_decide || case_match) =>//.
+      apply glob_def_genv_compat_struct in Heqo.
+      intro.
+      eapply elem_of_list_fmap_2 in H.
+      destruct H as [?[??]].
+      destruct x; simpl in H; subst.
+      econstructor; try eassumption.
+      by apply IHpath. }
+  Qed.
+*)
+End tu.
+
 #[global] Instance class_derives_here tu σ derived st :
   tu ⊧ σ ->
   TCEq (tu !! derived) (Some (Gstruct st)) ->
-  class_derives σ derived derived.
+  class_derives derived [].
 Proof.
   intros. eapply Derives_here, glob_def_genv_compat_struct.
   by apply (iffLR (TCEq_eq _ _)).
 Defined.
 
-#[global] Instance class_derives_base tu σ derived base st li result :
+#[global] Instance class_derives_base tu σ rest derived base st li :
   tu ⊧ σ ->
   TCEq (tu !! derived) (Some (Gstruct st)) ->
   TCElemOf (base, li) st.(s_bases) ->
-  class_derives σ base result ->
-  class_derives σ derived result.
+  class_derives base rest ->
+  class_derives derived (base :: rest).
 Proof.
   intros. eapply Derives_base; last done.
   - eapply glob_def_genv_compat_struct.
     by apply (iffLR (TCEq_eq _ _)).
-  - by apply (iffLR (elem_of_list_In _ _)), (iffLR (TCElemOf_iff _ _)).
+  - by apply (iffLR (TCElemOf_iff _ _)).
 Defined.
