theories/lang/cpp/logic/dispatch.v
@@ -17,28 +17,27 @@ Section with_cpp.
   Context `{Σ : cpp_logic}.
 
   (* the [offset] to cast a [base] to a [derived] *)
-  Fixpoint base_to_derived `(d : !class_derives σ derived base) : offset :=
-    match d with
-    | Derives_here st _ => o_id
-    | Derives_base base st _ _ _ _ d =>
-      o_dot (base_to_derived d) (o_derived σ base derived)
+  Fixpoint base_to_derived {σ : genv} (base : globname) (path : list globname) : offset :=
+    match path with
+    | nil => o_id
+    | derived :: rest => o_dot (o_derived σ base derived) (base_to_derived derived rest)
     end.
 
   (* the [offset] to cast a [derived] to a [base] *)
-  Fixpoint derived_to_base `(d : !class_derives σ derived base) : offset :=
-    match d with
-    | Derives_here st _ => o_id
-    | Derives_base base st _ _ _ _ d =>
-      o_dot (o_base σ derived base) (derived_to_base d)
+  Fixpoint derived_to_base {σ : genv} (derived : globname) (path : list globname) : offset :=
+    match path with
+    | nil => o_id
+    | base :: rest => o_dot (o_base σ derived base) (derived_to_base base rest)
     end.
 
   (** If successful, returns a pair of the function pointer to the
    *  implementation and the downcast for [this] pointer. *)
-  Definition get_impl `(r : !class_derives σ mdc tcls) (f : obj_name)
+  Definition get_impl {σ} (base : globname) (path : list globname) (f : obj_name)
     : option (ptr * offset) :=
-    let override := dispatch σ r f in
-    s ← override.(vimpl);
-    mret (_global s, base_to_derived override.(derivation)).
+    match dispatch.dispatch σ base path f with
+    | None => None
+    | Some (path, fptr) => Some (_global fptr, base_to_derived base path)
+    end.
 
   (** [resolve_virtual σ this cls f Q] returns [Q fa this'] if resolving [f] on
    * [this] results in a function that is equivalent to calling the pointer [fa]
@@ -47,20 +46,20 @@ Section with_cpp.
   Definition resolve_virtual {σ : genv}
              (this : ptr) (cls : globname) (f : obj_name)
              (Q : forall (faddr : ptr) (cls_type : globname) (this_addr : ptr), mpred) : mpred :=
-    Exists σ' mdc (pf : class_derives σ' mdc cls),
+    Exists σ' mdc (path : list globname),
+      [| class_derives cls path |] **
         (* ^ we quantify over another program environment because class
              extension is open, the caller does not need to know the target
              function.
            - the [class_derives] fact *must* be in [σ'] because [mdc] might
              not exist in [σ].
          *)
-    (Exists q, this |-> identityR (σ:=σ') cls (Some mdc) q  **
-                 [| class_compatible σ.(genv_tu) σ'.(genv_tu) cls |] ** True) //\\
+    (<absorb> Exists q, this |-> identityR (σ:=σ') cls path q) //\\
               (* ^ the [class_compatible σ σ' cls] ensures that the virtual
                    tables the [cls] class are compatible between the (possibly
                    different) translation units.
                *)
-      match get_impl pf f with
+      match get_impl cls path f with
       | Some (fa, off) => Q fa mdc (_offset_ptr this off)
       | None => (* the function wasn't found or the implementation was pure virtual *)
         False
