theories/lang/cpp/semantics/dispatch.v
@@ -1,5 +1,5 @@
 (*
- * Copyright (C) BedRock Systems Inc. 2020 Gregory Malecha
+ * Copyright (C) BedRock Systems Inc. 2020-2022
  *
  * SPDX-License-Identifier:AGPL-3.0-or-later
  *)
@@ -12,27 +12,27 @@ Require Import bedrock.lang.cpp.semantics.subtyping.
     1. Finding the correct function to invoke
     2. Fixing up the dispatch object.
     Consider the following example
-    [[
+    ```c++
     struct A { virtual void foo() = 0; };
     struct B : public A { virtual void foo() { } };
 
     A* a = new B();
     a->foo(); // same as [static_cast<B*>(a)->B::foo()]
-    ]]
+    ```
     note that in order to dispatch to the overridden function
-    the dispatch also introduces a [static_cast] to get a pointer
+    the dispatch also introduces a cast to get a pointer
     of the correct type.
  *)
-Record vhandle {σ : genv} : Set :=
+Record vhandle : Set :=
   { (* the name of the method that implements the function
        [None] means that there is no body.
      *)
     vimpl      : option obj_name
-  ; voverrider : globname
+  ; vpath      : list globname
+(*   ; voverrider : globname
   ; vfrom      : globname
   ; (* the cast for the [this] parameter *)
-    derivation : class_derives σ voverrider vfrom }.
-Arguments vhandle σ : clear implicits.
+    derivation : class_derives σ voverrider vfrom  *) }.
 
 Section dispatch.
   Context (σ : genv).
@@ -40,35 +40,35 @@ Section dispatch.
   Definition list_get {T} (t : obj_name) (l : list (obj_name * T)) : option T :=
     snd <$> List.find (fun '(t',_) => bool_decide (t = t')) l.
 
-  (** [dispatch' mdc from deriv final = (impl, cand)]
-      [impl] is the function to dispatch to and the fixup logic.
-      [cand] is the name of the implementation, which might be further overridden.
+  (** [dispatch base path fn = Some (impl_path, impl_fn)]
+      dispatches [fn] (the name of a member function on [Tnamed base])
+      given the path [path] (which is [mdc..base].
+      NOTE: [base] and [path] are the arguments to [identity]
+      - [impl_fn] is the name of the function to call
+      - [impl_path] is the path from (base..impl].
+      Some examples assuming:
+      ```c++
+      struct A { virtual void f(); };
+      struct B : public A { virtual void f(); };
+      struct C : public B { };
+      ```
+      - [dispatch "::A" ["::C","::B","::A"] "A::f()" = Some (["::B"], "B::f()")]
+      - [dispatch "::B" ["::C","::A"] "B::f()" = Some ([], "B::f()")]
    *)
-  #[local] Fixpoint dispatch' `(d : !class_derives σ mdc from) (final : obj_name)
-    : vhandle σ * obj_name :=
-    match d with
-    | Derives_here st _ =>
-      ({| vimpl := mjoin (list_get final st.(s_virtuals))
-        ; voverrider := mdc
-        ; vfrom := from
-        ; derivation := d |}, final)
-    | Derives_base base st _ _ _ _ d' =>
-      let result := dispatch' d' final in
-      match list_get result.2 st.(s_overrides) with
-      | None => result
-      | Some cand' =>
-        ({| vimpl := Some cand'
-          ; voverrider := mdc
-          ; vfrom := from
-          ; derivation := d |}, cand')
-      end
+  #[local] Fixpoint dispatch (base : globname) (path : list globname) (fn : obj_name)
+    : option (list globname * obj_name) :=
+    match path with
+    | nil => Some (path, fn)
+    | next :: rest =>
+        dispatch base rest fn ≫= fun '(hndl, override) =>
+          match σ.(genv_tu) !! next with
+          | Some (Gstruct st) =>
+              match list_get override st.(s_overrides) with
+              | Some cand' => Some (path, cand')
+              | None => Some (hndl, override)
+              end
+          | _ => None
+          end
     end.
-
-  (** [dispatch' mdc from deriv final] determines the function to
-      dispatch to and the fixup logic when calling [final] on an object
-      whose most derived class is [mdc].
-   *)
-  Definition dispatch `(d : !class_derives σ mdc from) (final : obj_name)
-    : vhandle σ := (dispatch' d final).1.
 
 End dispatch.
